specs/L2InteropHandler/L2InteropHandler/fun_formatEvmV1_user.lean
@@ -27,13 +27,13 @@ section
 
 open Clear EVMState Ast Expr Stmt FunctionDefinition State Interpreter ExecLemmas OutOfFuelLemmas Abstraction YulNotation PrimOps ReasoningPrinciple Utilities L2InteropHandler.Common generated.L2InteropHandler L2InteropHandler
 
-def A_fun_formatEvmV1 (var_3438_mpos : Identifier) (var_chainid var_addr : Literal) (s₀ s₉ : State) : Prop := sorry
+def A_fun_formatEvmV1 (var_3438_mpos : Identifier) (var_chainid var_addr : Literal) (s₀ s₉ : State) : Prop := fun_formatEvmV1_concrete_of_code.1 var_3438_mpos var_chainid var_addr s₀ s₉
 
 lemma fun_formatEvmV1_abs_of_concrete {s₀ s₉ : State} {var_3438_mpos var_chainid var_addr} :
   Spec (fun_formatEvmV1_concrete_of_code.1 var_3438_mpos var_chainid var_addr) s₀ s₉ →
   Spec (A_fun_formatEvmV1 var_3438_mpos var_chainid var_addr) s₀ s₉ := by
-  unfold fun_formatEvmV1_concrete_of_code A_fun_formatEvmV1
-  sorry
+  intro h
+  simpa [A_fun_formatEvmV1] using h
 
 end
 
