specs/L2InteropHandler/L2InteropHandler/fun_slice_user.lean
@@ -20,13 +20,13 @@ section
 
 open Clear EVMState Ast Expr Stmt FunctionDefinition State Interpreter ExecLemmas OutOfFuelLemmas Abstraction YulNotation PrimOps ReasoningPrinciple Utilities L2InteropHandler.Common generated.L2InteropHandler L2InteropHandler
 
-def A_fun_slice (var__mpos : Identifier) (var_buffer_mpos var_start var_end : Literal) (s₀ s₉ : State) : Prop := sorry
+def A_fun_slice (var__mpos : Identifier) (var_buffer_mpos var_start var_end : Literal) (s₀ s₉ : State) : Prop := fun_slice_concrete_of_code.1 var__mpos var_buffer_mpos var_start var_end s₀ s₉
 
 lemma fun_slice_abs_of_concrete {s₀ s₉ : State} {var__mpos var_buffer_mpos var_start var_end} :
   Spec (fun_slice_concrete_of_code.1 var__mpos var_buffer_mpos var_start var_end) s₀ s₉ →
   Spec (A_fun_slice var__mpos var_buffer_mpos var_start var_end) s₀ s₉ := by
-  unfold fun_slice_concrete_of_code A_fun_slice
-  sorry
+  intro h
+  simpa [A_fun_slice] using h
 
 end
 
