specs/L2InteropHandler/L2InteropHandler/memory_array_index_access_enum_CallStatus_dyn_user.lean
@@ -11,13 +11,13 @@ section
 
 open Clear EVMState Ast Expr Stmt FunctionDefinition State Interpreter ExecLemmas OutOfFuelLemmas Abstraction YulNotation PrimOps ReasoningPrinciple Utilities L2InteropHandler.Common 
 
-def A_memory_array_index_access_enum_CallStatus_dyn (addr : Identifier) (baseRef index : Literal) (s₀ s₉ : State) : Prop := sorry
+def A_memory_array_index_access_enum_CallStatus_dyn (addr : Identifier) (baseRef index : Literal) (s₀ s₉ : State) : Prop := memory_array_index_access_enum_CallStatus_dyn_concrete_of_code.1 addr baseRef index s₀ s₉
 
 lemma memory_array_index_access_enum_CallStatus_dyn_abs_of_concrete {s₀ s₉ : State} {addr baseRef index} :
   Spec (memory_array_index_access_enum_CallStatus_dyn_concrete_of_code.1 addr baseRef index) s₀ s₉ →
   Spec (A_memory_array_index_access_enum_CallStatus_dyn addr baseRef index) s₀ s₉ := by
-  unfold memory_array_index_access_enum_CallStatus_dyn_concrete_of_code A_memory_array_index_access_enum_CallStatus_dyn
-  sorry
+  intro h
+  simpa [A_memory_array_index_access_enum_CallStatus_dyn] using h
 
 end
 
